rt haskell+refine+crefine: prove handleRecv_ccorres and handleSyscall_ccorres
Signed-off-by: Michael McInerney <michael.mcinerney@proofcraft.systems>

spec/haskell/src/SEL4.lhs
@@ -22,7 +22,8 @@ This is the top-level module; it defines the interface between the kernel and th
 > import SEL4.API.Types
 > import SEL4.Kernel.CSpace(lookupCap)
 > import SEL4.Kernel.Thread(schedule, activateThread)
-> import SEL4.Model.StateData(KernelState, Kernel, getCurThread, doMachineOp, stateAssert, rct_imp_activatable'_asrt, cur_tcb'_asrt)
+> import SEL4.Model.StateData(KernelState, Kernel, getCurThread, doMachineOp, stateAssert,
+>                             rct_imp_activatable'_asrt, cur_tcb'_asrt, weak_sch_act_wf_asrt)
 > import SEL4.Model.Preemption(withoutPreemption)
 > import SEL4.Object.Structures
 > import SEL4.Object.TCB(asUser, mcsPreemptionPoint)
@@ -41,6 +42,7 @@ faults, and system calls; the set of possible events is defined in
 > callKernel ev = do
 >     stateAssert fastpathKernelAssertions ""
 >     stateAssert cur_tcb'_asrt "`cur_tcb'`"
+>     stateAssert weak_sch_act_wf_asrt ""
 >     runExceptT $ handleEvent ev
 >         `catchError` (\_ -> withoutPreemption $ do
 >                       mcsPreemptionPoint
